minor

src/prop/PFCertify.v
@@ -23,422 +23,430 @@ Require Import Global.
 Require Import Local.
 Require Import Thread.
 
+Set Implicit Arguments.
 
-Section PFCertify.
-  Variable lang: language.
 
-  Variant pf_certify (loc: Loc.t) (th: Thread.t lang): Prop :=
-    | pf_certify_failure
-        pf e th1 th2
-        (STEPS: rtc (tau (Thread.step (Global.max_reserved (Thread.global th)) true)) th th1)
-        (STEP_FAILURE: Thread.step (Global.max_reserved (Thread.global th)) pf e th1 th2)
-        (EVENT_FAILURE: ThreadEvent.get_machine_event e = MachineEvent.failure)
-    | pf_certify_fulfill
-        pf e th1 th2
-        from to val released ord
-        (STEPS: rtc (tau (Thread.step (Global.max_reserved (Thread.global th)) true)) th th1)
-        (STEP_FULFILL: Thread.step (Global.max_reserved (Thread.global th)) pf e th1 th2)
-        (EVENT_FULFILL: ThreadEvent.is_writing e = Some (loc, from, to, val, released, ord))
-        (TO: Time.lt (Memory.max_ts loc (Global.memory (Thread.global th1))) to)
-        (ORD: Ordering.le ord Ordering.na)
-  .
+Module PFCertify.
+  Section PFCertify.
+    Variable lang: language.
 
-  Variant pf_certify_aux (reserved: OptTimeMap.t) (loc: Loc.t) (th: Thread.t lang): Prop :=
-    | pf_certify_aux_failure
-        pf e th1 th2
-        (STEPS: rtc (tau (Thread.step reserved true)) th th1)
-        (STEP_FAILURE: Thread.step reserved pf e th1 th2)
-        (EVENT_FAILURE: ThreadEvent.get_machine_event e = MachineEvent.failure)
-    | pf_certify_aux_fulfill
-        pf e th1 th2
-        from to val released ord
-        (STEPS: rtc (tau (Thread.step reserved true)) th th1)
-        (STEP_FULFILL: Thread.step reserved pf e th1 th2)
-        (EVENT_FULFILL: ThreadEvent.is_writing e = Some (loc, from, to, val, released, ord))
-        (TO: Time.lt (Memory.max_ts loc (Global.memory (Thread.global th1))) to)
-        (ORD: Ordering.le ord Ordering.na)
-  .
+    Variant pf_certify (loc: Loc.t) (th: Thread.t lang): Prop :=
+      | pf_certify_failure
+          pf e th1 th2
+          (STEPS: rtc (tau (Thread.step (Global.max_reserved (Thread.global th)) true)) th th1)
+          (STEP_FAILURE: Thread.step (Global.max_reserved (Thread.global th)) pf e th1 th2)
+          (EVENT_FAILURE: ThreadEvent.get_machine_event e = MachineEvent.failure)
+      | pf_certify_fulfill
+          pf e th1 th2
+          from to val released ord
+          (STEPS: rtc (tau (Thread.step (Global.max_reserved (Thread.global th)) true)) th th1)
+          (STEP_FULFILL: Thread.step (Global.max_reserved (Thread.global th)) pf e th1 th2)
+          (EVENT_FULFILL: ThreadEvent.is_writing e = Some (loc, from, to, val, released, ord))
+          (TO: Time.lt (Memory.max_ts loc (Global.memory (Thread.global th1))) to)
+          (ORD: Ordering.le ord Ordering.na)
+    .
 
-  Definition non_sc (e: ThreadEvent.t): Prop :=
-    ~ ThreadEvent.is_sc e /\ ThreadEvent.get_machine_event e = MachineEvent.silent.
+    Variant pf_certify_aux (reserved: OptTimeMap.t) (loc: Loc.t) (th: Thread.t lang): Prop :=
+      | pf_certify_aux_failure
+          pf e th1 th2
+          (STEPS: rtc (tau (Thread.step reserved true)) th th1)
+          (STEP_FAILURE: Thread.step reserved pf e th1 th2)
+          (EVENT_FAILURE: ThreadEvent.get_machine_event e = MachineEvent.failure)
+      | pf_certify_aux_fulfill
+          pf e th1 th2
+          from to val released ord
+          (STEPS: rtc (tau (Thread.step reserved true)) th th1)
+          (STEP_FULFILL: Thread.step reserved pf e th1 th2)
+          (EVENT_FULFILL: ThreadEvent.is_writing e = Some (loc, from, to, val, released, ord))
+          (TO: Time.lt (Memory.max_ts loc (Global.memory (Thread.global th1))) to)
+          (ORD: Ordering.le ord Ordering.na)
+    .
 
-  Variant certify (reserved: OptTimeMap.t) (loc: Loc.t) (th: Thread.t lang): Prop :=
-    | certify_failure
-        pf e th1 th2
-        (STEPS: rtc (pstep (Thread.step_allpf reserved) non_sc) th th1)
-        (STEP_FAILURE: Thread.step reserved pf e th1 th2)
-        (EVENT_FAILURE: ThreadEvent.get_machine_event e = MachineEvent.failure)
-    | certify_fulfill
-        pf e th1 th2
-        from to val released ord
-        (STEPS: rtc (pstep (Thread.step_allpf reserved) non_sc) th th1)
-        (STEP_FULFILL: Thread.step reserved pf e th1 th2)
-        (EVENT_FULFILL: ThreadEvent.is_writing e = Some (loc, from, to, val, released, ord))
-        (TO: Time.lt (Memory.max_ts loc (Global.memory (Thread.global th1))) to)
-        (ORD: Ordering.le ord Ordering.na)
-  .
+    Definition non_sc (e: ThreadEvent.t): Prop :=
+      ~ ThreadEvent.is_sc e /\ ThreadEvent.get_machine_event e = MachineEvent.silent.
 
-  Variant non_sc_consistent (th: Thread.t lang): Prop :=
-    | non_sc_consistent_failure
-        pf e th1 th2
-        (STEPS: rtc (pstep (Thread.step_allpf (Global.max_reserved (Thread.global th))) non_sc) th th1)
-        (STEP_FAILURE: Thread.step (Global.max_reserved (Thread.global th)) pf e th1 th2)
-        (EVENT_FAILURE: ThreadEvent.get_machine_event e = MachineEvent.failure)
-    | non_sc_consistent_promises
-        th2
-        (STEPS: rtc (pstep (Thread.step_allpf (Global.max_reserved (Thread.global th))) non_sc) th th2)
-        (PROMISES: Local.promises (Thread.local th2) = BoolMap.bot)
-  .
+    Variant certify (reserved: OptTimeMap.t) (loc: Loc.t) (th: Thread.t lang): Prop :=
+      | certify_failure
+          pf e th1 th2
+          (STEPS: rtc (pstep (Thread.step_allpf reserved) non_sc) th th1)
+          (STEP_FAILURE: Thread.step reserved pf e th1 th2)
+          (EVENT_FAILURE: ThreadEvent.get_machine_event e = MachineEvent.failure)
+      | certify_fulfill
+          pf e th1 th2
+          from to val released ord
+          (STEPS: rtc (pstep (Thread.step_allpf reserved) non_sc) th th1)
+          (STEP_FULFILL: Thread.step reserved pf e th1 th2)
+          (EVENT_FULFILL: ThreadEvent.is_writing e = Some (loc, from, to, val, released, ord))
+          (TO: Time.lt (Memory.max_ts loc (Global.memory (Thread.global th1))) to)
+          (ORD: Ordering.le ord Ordering.na)
+    .
 
-  Lemma rtc_tau_step_rtc_non_sc_step
-        reserved (th1 th2: Thread.t lang)
-        (STEPS: rtc (Thread.tau_step reserved) th1 th2):
-    exists th2',
-      (<<STEPS1: rtc (pstep (Thread.step_allpf reserved) non_sc) th1 th2'>>) /\
-      ((<<TH2: th2' = th2>>) \/
-       (<<STEPS2: rtc (Thread.tau_step reserved) th2' th2>>) /\
-       (<<PROMISES: Local.promises (Thread.local th2') = BoolMap.bot>>)).
-  Proof.
-    induction STEPS.
-    { esplits; eauto. }
-    inv H. inv TSTEP.
-    destruct (classic (ThreadEvent.is_sc e)).
-    - esplits; [refl|]. right. split.
-      + econs 2; eauto. econs; eauto.
-      + inv STEP; inv STEP0; ss. inv LOCAL. auto.
-    - des.
-      + esplits; [|eauto]. econs 2; eauto.
-        econs; eauto. destruct e; ss.
-      + esplits; [|eauto]. econs 2; eauto.
-        econs; eauto. destruct e; ss.
-  Qed.
+    Variant non_sc_consistent (th: Thread.t lang): Prop :=
+      | non_sc_consistent_failure
+          pf e th1 th2
+          (STEPS: rtc (pstep (Thread.step_allpf (Global.max_reserved (Thread.global th))) non_sc) th th1)
+          (STEP_FAILURE: Thread.step (Global.max_reserved (Thread.global th)) pf e th1 th2)
+          (EVENT_FAILURE: ThreadEvent.get_machine_event e = MachineEvent.failure)
+      | non_sc_consistent_promises
+          th2
+          (STEPS: rtc (pstep (Thread.step_allpf (Global.max_reserved (Thread.global th))) non_sc) th th2)
+          (PROMISES: Local.promises (Thread.local th2) = BoolMap.bot)
+    .
 
-  Lemma consistent_non_sc_consistent
-        th
-        (CONS: Thread.consistent th):
-    non_sc_consistent th.
-  Proof.
-    inv CONS.
-    - inv FAILURE.
-      exploit rtc_tau_step_rtc_non_sc_step; eauto. i. des.
-      + subst. econs 1; eauto.
-      + econs 2; eauto.
-    - exploit rtc_tau_step_rtc_non_sc_step; eauto. i. des.
-      + subst. econs 2; eauto.
-      + econs 2; eauto.
-  Qed.
+    Lemma rtc_tau_step_rtc_non_sc_step
+          reserved (th1 th2: Thread.t lang)
+          (STEPS: rtc (Thread.tau_step reserved) th1 th2):
+      exists th2',
+        (<<STEPS1: rtc (pstep (Thread.step_allpf reserved) non_sc) th1 th2'>>) /\
+        ((<<TH2: th2' = th2>>) \/
+         (<<STEPS2: rtc (Thread.tau_step reserved) th2' th2>>) /\
+         (<<PROMISES: Local.promises (Thread.local th2') = BoolMap.bot>>)).
+    Proof.
+      induction STEPS.
+      { esplits; eauto. }
+      inv H. inv TSTEP.
+      destruct (classic (ThreadEvent.is_sc e)).
+      - esplits; [refl|]. right. split.
+        + econs 2; eauto. econs; eauto.
+        + inv STEP; inv STEP0; ss. inv LOCAL. auto.
+      - des.
+        + esplits; [|eauto]. econs 2; eauto.
+          econs; eauto. destruct e; ss.
+        + esplits; [|eauto]. econs 2; eauto.
+          econs; eauto. destruct e; ss.
+    Qed.
 
-  Lemma non_sc_consistent_certify
-        th loc
-        (LC_WF: Local.wf (Thread.local th) (Thread.global th))
-        (GL_WF: Global.wf (Thread.global th))
-        (CONS: non_sc_consistent th)
-        (PROMISED: Local.promises (Thread.local th) loc = true):
-    certify (Global.max_reserved (Thread.global th)) loc th.
-  Proof.
-    inv CONS.
-    { econs 1; eauto. }
-    remember (Global.max_reserved (Thread.global th)) as reserved.
-    clear Heqreserved. revert PROMISED.
-    induction STEPS; i.
-    { rewrite PROMISES in *. ss. }
-    destruct (Local.promises (Thread.local y) loc) eqn:PROMISEDY.
-    { dup H. inv H0. inv STEP.
-      exploit Thread.step_future; try exact STEP; eauto. i. des.
-      exploit IHSTEPS; eauto. i. inv x1.
-      - econs 1; try exact STEP_FAILURE; eauto.
-      - econs 2; try exact STEP_FULFILL; eauto.
-    }
+    Lemma consistent_non_sc_consistent
+          th
+          (CONS: Thread.consistent th):
+      non_sc_consistent th.
+    Proof.
+      inv CONS.
+      - inv FAILURE.
+        exploit rtc_tau_step_rtc_non_sc_step; eauto. i. des.
+        + subst. econs 1; eauto.
+        + econs 2; eauto.
+      - exploit rtc_tau_step_rtc_non_sc_step; eauto. i. des.
+        + subst. econs 2; eauto.
+        + econs 2; eauto.
+    Qed.
 
-    move PROMISEDY at bottom.
-    inv H. inv STEP.
-    inv STEP0; inv STEP; ss; (try congr); (try by inv LOCAL; ss; congr).
-    { (* promise *)
-      inv LOCAL. inv PROMISE. ss.
-      exploit BoolMap.add_le; try exact ADD; eauto. i. congr.
-    }
-
-    { (* write *)
-      assert (loc0 = loc /\ Ordering.le ord Ordering.na).
-      { inv LOCAL. inv FULFILL; ss; try congr. split; ss.
-        revert PROMISEDY. erewrite BoolMap.remove_o; eauto.
-        condtac; ss. congr.
-      }
-      des. subst.
-      destruct (TimeFacts.le_lt_dec to (Memory.max_ts loc (Global.memory gl1))); cycle 1.
-      { econs 2; [refl|..].
-        - econs 2; [|econs 3]; eauto.
-        - ss.
-        - ss.
-        - ss.
-      }
-
-      exploit (Memory.max_ts_spec loc); try apply GL_WF. i. des.
-      destruct msg. clear MAX.
-      econs 1; [refl|..].
-      - econs 2; [|econs 9]; eauto.
-        econs. econs 2; eauto.
-        + unfold TView.racy_view.
-          eapply TimeFacts.lt_le_lt; eauto.
-          inv LOCAL. inv WRITABLE. ss.
-          eapply TimeFacts.le_lt_lt; eauto.
-          apply LC_WF.
-        + destruct ord; ss.
-      - ss.
-    }
-
-    { (* update *)
-      assert (Ordering.le ordw Ordering.na).
-      { inv LOCAL1. inv LOCAL2.  inv FULFILL; ss; try congr. }
-      econs 1; [refl|..].
-      - econs 2; [|econs 10]; eauto.
-      - ss.
-    }
-  Qed.
-
-  Variant pf_sim_thread (th_src th_tgt: Thread.t lang): Prop :=
-    | pf_sim_thread_intro
-        (STATE: Thread.state th_src = Thread.state th_tgt)
-        (TVIEW: Local.tview (Thread.local th_src) = Local.tview (Thread.local th_tgt))
-        (SC: Global.sc (Thread.global th_src) = Global.sc (Thread.global th_tgt))
-        (PROMISES: BoolMap.minus (Global.promises (Thread.global th_src)) (Local.promises (Thread.local th_src)) =
-                   BoolMap.minus (Global.promises (Thread.global th_tgt)) (Local.promises (Thread.local th_tgt)))
-        (RESERVES: BoolMap.minus (Global.reserves (Thread.global th_src)) (Local.reserves (Thread.local th_src)) =
-                   BoolMap.minus (Global.reserves (Thread.global th_tgt)) (Local.reserves (Thread.local th_tgt)))
-        (MEMORY: Global.memory (Thread.global th_src) = Global.memory (Thread.global th_tgt))
-  .
-
-  Program Instance pf_sim_thread_Equivalence: Equivalence pf_sim_thread.
-  Next Obligation.
-    ii. econs; ss.
-  Qed.
-  Next Obligation.
-    ii. inv H. ss.
-  Qed.
-  Next Obligation.
-    ii. inv H. inv H0. econs; try congr.
-  Qed.
-
-  Lemma pf_sim_thread_internal_step
-        th1_src
-        reserved e th1_tgt th2_tgt
-        (SIM1: pf_sim_thread th1_src th1_tgt)
-        (STEP_TGT: Thread.step reserved false e th1_tgt th2_tgt):
-    pf_sim_thread th1_src th2_tgt.
-  Proof.
-    inv SIM1. inv STEP_TGT. ss. inv STEP.
-    - inv LOCAL. econs; ss.
-      rewrite PROMISES.
-      eauto using Promises.promise_minus.
-    - inv LOCAL. econs; ss.
-      rewrite RESERVES.
-      eauto using Reserves.reserve_minus.
-    - inv LOCAL. econs; ss.
-      rewrite RESERVES.
-      eauto using Reserves.cancel_minus.
-  Qed.
-
-  Lemma sim_is_racy
-        lc_src gl_src lc_tgt gl_tgt
-        loc to ord
-        (TVIEW: Local.tview lc_src = Local.tview lc_tgt)
-        (PROMISES: BoolMap.minus (Global.promises gl_src) (Local.promises lc_src) =
-                   BoolMap.minus (Global.promises gl_tgt) (Local.promises lc_tgt))
-        (MEMORY: Global.memory gl_src = Global.memory gl_tgt)
-        (RACE_TGT: Local.is_racy lc_tgt gl_tgt loc to ord):
-    Local.is_racy lc_src gl_src loc to ord.
-  Proof.
-    inv RACE_TGT.
-    - eapply equal_f in PROMISES.
-      unfold BoolMap.minus in *.
-      rewrite GET, GETP in *. ss.
-      destruct (Global.promises gl_src loc) eqn:GRSV; ss.
-      destruct (Local.promises lc_src loc) eqn:RSV; ss.
-      econs 1; eauto.
-    - rewrite <- TVIEW, <- MEMORY in *. eauto.
-  Qed.
-
-  Lemma pf_sim_thread_program_step
-        (reserved: OptTimeMap.t)
-        th1_src
-        e th1_tgt th2_tgt
-        (RESERVED: forall loc, reserved loc <-> Global.reserves (Thread.global th1_src) loc)
-        (SIM1: pf_sim_thread th1_src th1_tgt)
-        (STEP_TGT: Thread.step reserved true e th1_tgt th2_tgt)
-        (NONSC: ~ ThreadEvent.is_sc e):
-    exists th2_src,
-      (<<STEP_SRC: Thread.step reserved true e th1_src th2_src>>) /\
-      (<<SIM2: pf_sim_thread th2_src th2_tgt>>).
-  Proof.
-    destruct th1_src as [st1_src [tview1_src prm1_src rsv1_src] [sc1_src gprm1_src grsv1_src mem1_src]],
-        th1_tgt as [st1_tgt [tview1_tgt prm1_tgt rsv1_tgt] [sc1_tgt gprm1_tgt grsv1_tgt mem1_tgt]].
-    inv SIM1. ss. subst.
-    inv STEP_TGT. inv STEP; ss.
-    { (* silent *)
-      esplits.
-      - econs; [|econs 1]; eauto.
-      - ss.
-    }
-    { (* read *)
-      inv LOCAL. ss.
-      esplits.
-      - econs; [|econs 2]; eauto.
-      - ss.
-    }
-    { (* write *)
-      inv LOCAL. ss.
-      esplits.
-      - econs; [|econs 3]; eauto.
-        econs; s; eauto. i.
-        exploit NON_RESERVED; eauto. i. des; auto.
-        specialize (RESERVED loc). rewrite GET in *.
-        destruct (grsv1_src loc) eqn:GRSV_SRC; ss; try by intuition.
-        destruct (rsv1_src loc) eqn:RSV_SRC; auto.
-        eapply equal_f in RESERVES.
-        unfold BoolMap.minus in RESERVES.
-        rewrite GRSV_SRC, RSV_SRC, x0 in RESERVES. ss.
-        destruct (grsv1_tgt loc); ss.
-      - econs; ss.
-        rewrite PROMISES.
-        eauto using Promises.fulfill_minus.
-    }
-    { (* update *)
-      inv LOCAL1. inv LOCAL2. ss.
-      esplits.
-      - econs; [|econs 4]; eauto.
-        econs; s; eauto. i.
-        exploit NON_RESERVED; eauto. i. des; auto.
-        specialize (RESERVED loc). rewrite GET0 in *.
-        destruct (grsv1_src loc) eqn:GRSV_SRC; ss; try by intuition.
-        destruct (rsv1_src loc) eqn:RSV_SRC; auto.
-        eapply equal_f in RESERVES.
-        unfold BoolMap.minus in RESERVES.
-        rewrite GRSV_SRC, RSV_SRC, x0 in RESERVES. ss.
-        destruct (grsv1_tgt loc); ss.
-      - econs; ss.
-        rewrite PROMISES.
-        eauto using Promises.fulfill_minus.
-    }
-    { (* fence *)
-      inv LOCAL. ss.
-      esplits.
-      - econs; [|econs 5]; eauto. econs; ss.
-      - ss.
-    }
-    { (* failure *)
-      inv LOCAL. ss.
-      esplits.
-      - econs; [|econs 7]; eauto.
-      - ss.
-    }
-    { (* racy read *)
-      inv LOCAL. ss.
-      esplits.
-      - econs; [|econs 8]; eauto.
-        econs. eapply sim_is_racy; try eapply RACE; ss.
-      - ss.
-    }
-    { (* racy write *)
-      inv LOCAL. ss.
-      esplits.
-      - econs; [|econs 9]; eauto.
-        econs. eapply sim_is_racy; try eapply RACE; ss.
-      - ss.
-    }
-    { (* racy update *)
-      esplits.
-      - econs; [|econs 10]; eauto.
-        inv LOCAL.
-        + econs 1. ss.
-        + econs 2. ss.
-        + econs 3. eapply sim_is_racy; try eapply RACE; ss.
-      - ss.
-    }
-  Qed.
-
-  Lemma program_step_reserves
-        reserved e (th1 th2: Thread.t lang)
-        (STEP: Thread.step reserved true e th1 th2):
-    Global.reserves (Thread.global th1) = Global.reserves (Thread.global th2).
-  Proof.
-    inv STEP. inv STEP0; ss; try by (inv LOCAL; ss).
-    inv LOCAL1. inv LOCAL2. ss.
-  Qed.
-
-  Lemma certify_pf_certify_aux
-        (reserved: OptTimeMap.t)
-        th_src th_tgt loc
-        (SIM: pf_sim_thread th_src th_tgt)
-        (RESERVED: forall loc, reserved loc <-> Global.reserves (Thread.global th_src) loc)
-        (CERTIFY: certify reserved loc th_tgt):
-    pf_certify_aux reserved loc th_src.
-  Proof.
-    inv CERTIFY.
-    { revert th_src SIM RESERVED.
+    Lemma non_sc_consistent_certify
+          th loc
+          (LC_WF: Local.wf (Thread.local th) (Thread.global th))
+          (GL_WF: Global.wf (Thread.global th))
+          (CONS: non_sc_consistent th)
+          (PROMISED: Local.promises (Thread.local th) loc = true):
+      certify (Global.max_reserved (Thread.global th)) loc th.
+    Proof.
+      inv CONS.
+      { econs 1; eauto. }
+      remember (Global.max_reserved (Thread.global th)) as reserved.
+      clear Heqreserved. revert PROMISED.
       induction STEPS; i.
-      { destruct pf; [|inv STEP_FAILURE; inv STEP; ss].
-        exploit pf_sim_thread_program_step; try exact STEP_FAILURE; eauto.
-        { destruct e; ss. }
-        i. des.
-        econs 1; [refl|..]; eauto.
-      }
-      inv H. inv STEP. destruct pf0.
-      { exploit pf_sim_thread_program_step; try exact STEP0; eauto; try apply EVENT. i. des.
-        exploit IHSTEPS; eauto.
-        { i. erewrite <- program_step_reserves; eauto. }
-        i. inv x1.
-        - econs 1; try exact STEP_FAILURE0; eauto.
-          econs 2; eauto. econs; eauto. apply EVENT.
-        - econs 2; try exact STEP_FULFILL; eauto.
-          econs 2; eauto. econs; eauto. apply EVENT.
-      }
-      { eauto using pf_sim_thread_internal_step. }
-    }
-    { revert th_src SIM RESERVED.
-      induction STEPS; i.
-      { destruct pf; [|inv STEP_FULFILL; inv STEP; ss].
-        exploit pf_sim_thread_program_step; try exact STEP_FAILURE; eauto.
-        { destruct e; ss. }
-        i. des.
-        econs 2; [refl|..]; eauto.
-        inv SIM. congr.
-      }
-      inv H. inv STEP. destruct pf0.
-      { exploit pf_sim_thread_program_step; try exact STEP0; eauto; try apply EVENT. i. des.
-        exploit IHSTEPS; eauto.
-        { i. erewrite <- program_step_reserves; eauto. }
-        i. inv x1.
+      { rewrite PROMISES in *. ss. }
+      destruct (Local.promises (Thread.local y) loc) eqn:PROMISEDY.
+      { dup H. inv H0. inv STEP.
+        exploit Thread.step_future; try exact STEP; eauto. i. des.
+        exploit IHSTEPS; eauto. i. inv x1.
         - econs 1; try exact STEP_FAILURE; eauto.
-          econs 2; eauto. econs; eauto. apply EVENT.
-        - econs 2; try exact STEP_FULFILL0; eauto.
-          econs 2; eauto. econs; eauto. apply EVENT.
+        - econs 2; try exact STEP_FULFILL; eauto.
       }
-      { eauto using pf_sim_thread_internal_step. }
-    }
-  Qed.
 
-  Lemma certify_pf_certify
-        th loc
-        (CERTIFY: certify (Global.max_reserved (Thread.global th)) loc th):
-    pf_certify loc th.
-  Proof.
-    exploit certify_pf_certify_aux; try exact CERTIFY; try refl.
-    { i. unfold Global.max_reserved, Memory.max_opt_timemap. condtac; ss. }
-    i. inv x0.
-    - econs 1; eauto.
-    - econs 2; eauto.
-  Qed.
+      move PROMISEDY at bottom.
+      inv H. inv STEP.
+      inv STEP0; inv STEP; ss; (try congr); (try by inv LOCAL; ss; congr).
+      { (* promise *)
+        inv LOCAL. inv PROMISE. ss.
+        exploit BoolMap.add_le; try exact ADD; eauto. i. congr.
+      }
 
-  Lemma consistent_pf_certify
-        th loc
-        (LC_WF: Local.wf (Thread.local th) (Thread.global th))
-        (GL_WF: Global.wf (Thread.global th))
-        (CONS: Thread.consistent th)
-        (PROMISED: th.(Thread.local).(Local.promises) loc = true):
-    pf_certify loc th.
-  Proof.
-    apply certify_pf_certify; auto.
-    apply non_sc_consistent_certify; auto.
-    apply consistent_non_sc_consistent; auto.
-  Qed.
+      { (* write *)
+        assert (loc0 = loc /\ Ordering.le ord Ordering.na).
+        { inv LOCAL. inv FULFILL; ss; try congr. split; ss.
+          revert PROMISEDY. erewrite BoolMap.remove_o; eauto.
+          condtac; ss. congr.
+        }
+        des. subst.
+        destruct (TimeFacts.le_lt_dec to (Memory.max_ts loc (Global.memory gl1))); cycle 1.
+        { econs 2; [refl|..].
+          - econs 2; [|econs 3]; eauto.
+          - ss.
+          - ss.
+          - ss.
+        }
+
+        exploit (Memory.max_ts_spec loc); try apply GL_WF. i. des.
+        destruct msg. clear MAX.
+        econs 1; [refl|..].
+        - econs 2; [|econs 9]; eauto.
+          econs. econs 2; eauto.
+          + unfold TView.racy_view.
+            eapply TimeFacts.lt_le_lt; eauto.
+            inv LOCAL. inv WRITABLE. ss.
+            eapply TimeFacts.le_lt_lt; eauto.
+            apply LC_WF.
+          + destruct ord; ss.
+        - ss.
+      }
+
+      { (* update *)
+        assert (Ordering.le ordw Ordering.na).
+        { inv LOCAL1. inv LOCAL2.  inv FULFILL; ss; try congr. }
+        econs 1; [refl|..].
+        - econs 2; [|econs 10]; eauto.
+        - ss.
+      }
+    Qed.
+
+    Variant sim_thread (th_src th_tgt: Thread.t lang): Prop :=
+      | sim_thread_intro
+          (STATE: Thread.state th_src = Thread.state th_tgt)
+          (TVIEW: Local.tview (Thread.local th_src) = Local.tview (Thread.local th_tgt))
+          (SC: Global.sc (Thread.global th_src) = Global.sc (Thread.global th_tgt))
+          (PROMISES: BoolMap.minus (Global.promises (Thread.global th_src))
+                                   (Local.promises (Thread.local th_src)) =
+                     BoolMap.minus (Global.promises (Thread.global th_tgt))
+                                   (Local.promises (Thread.local th_tgt)))
+          (RESERVES: BoolMap.minus (Global.reserves (Thread.global th_src))
+                                   (Local.reserves (Thread.local th_src)) =
+                     BoolMap.minus (Global.reserves (Thread.global th_tgt))
+                                   (Local.reserves (Thread.local th_tgt)))
+          (MEMORY: Global.memory (Thread.global th_src) = Global.memory (Thread.global th_tgt))
+    .
+
+    Program Instance sim_thread_Equivalence: Equivalence sim_thread.
+    Next Obligation.
+      ii. econs; ss.
+    Qed.
+    Next Obligation.
+      ii. inv H. ss.
+    Qed.
+    Next Obligation.
+      ii. inv H. inv H0. econs; try congr.
+    Qed.
+
+    Lemma sim_thread_internal_step
+          th1_src
+          reserved e th1_tgt th2_tgt
+          (SIM1: sim_thread th1_src th1_tgt)
+          (STEP_TGT: Thread.step reserved false e th1_tgt th2_tgt):
+      sim_thread th1_src th2_tgt.
+    Proof.
+      inv SIM1. inv STEP_TGT. ss. inv STEP.
+      - inv LOCAL. econs; ss.
+        rewrite PROMISES.
+        eauto using Promises.promise_minus.
+      - inv LOCAL. econs; ss.
+        rewrite RESERVES.
+        eauto using Reserves.reserve_minus.
+      - inv LOCAL. econs; ss.
+        rewrite RESERVES.
+        eauto using Reserves.cancel_minus.
+    Qed.
+
+    Lemma sim_is_racy
+          lc_src gl_src lc_tgt gl_tgt
+          loc to ord
+          (TVIEW: Local.tview lc_src = Local.tview lc_tgt)
+          (PROMISES: BoolMap.minus (Global.promises gl_src) (Local.promises lc_src) =
+                     BoolMap.minus (Global.promises gl_tgt) (Local.promises lc_tgt))
+          (MEMORY: Global.memory gl_src = Global.memory gl_tgt)
+          (RACE_TGT: Local.is_racy lc_tgt gl_tgt loc to ord):
+      Local.is_racy lc_src gl_src loc to ord.
+    Proof.
+      inv RACE_TGT.
+      - eapply equal_f in PROMISES.
+        unfold BoolMap.minus in *.
+        rewrite GET, GETP in *. ss.
+        destruct (Global.promises gl_src loc) eqn:GRSV; ss.
+        destruct (Local.promises lc_src loc) eqn:RSV; ss.
+        econs 1; eauto.
+      - rewrite <- TVIEW, <- MEMORY in *. eauto.
+    Qed.
+
+    Lemma sim_thread_program_step
+          (reserved: OptTimeMap.t)
+          th1_src
+          e th1_tgt th2_tgt
+          (RESERVED: forall loc, reserved loc <-> Global.reserves (Thread.global th1_src) loc)
+          (SIM1: sim_thread th1_src th1_tgt)
+          (STEP_TGT: Thread.step reserved true e th1_tgt th2_tgt)
+          (NONSC: ~ ThreadEvent.is_sc e):
+      exists th2_src,
+        (<<STEP_SRC: Thread.step reserved true e th1_src th2_src>>) /\
+        (<<SIM2: sim_thread th2_src th2_tgt>>).
+    Proof.
+      destruct th1_src as [st1_src [tview1_src prm1_src rsv1_src] [sc1_src gprm1_src grsv1_src mem1_src]],
+          th1_tgt as [st1_tgt [tview1_tgt prm1_tgt rsv1_tgt] [sc1_tgt gprm1_tgt grsv1_tgt mem1_tgt]].
+      inv SIM1. ss. subst.
+      inv STEP_TGT. inv STEP; ss.
+      { (* silent *)
+        esplits.
+        - econs; [|econs 1]; eauto.
+        - ss.
+      }
+      { (* read *)
+        inv LOCAL. ss.
+        esplits.
+        - econs; [|econs 2]; eauto.
+        - ss.
+      }
+      { (* write *)
+        inv LOCAL. ss.
+        esplits.
+        - econs; [|econs 3]; eauto.
+          econs; s; eauto. i.
+          exploit NON_RESERVED; eauto. i. des; auto.
+          specialize (RESERVED loc). rewrite GET in *.
+          destruct (grsv1_src loc) eqn:GRSV_SRC; ss; try by intuition.
+          destruct (rsv1_src loc) eqn:RSV_SRC; auto.
+          eapply equal_f in RESERVES.
+          unfold BoolMap.minus in RESERVES.
+          rewrite GRSV_SRC, RSV_SRC, x0 in RESERVES. ss.
+          destruct (grsv1_tgt loc); ss.
+        - econs; ss.
+          rewrite PROMISES.
+          eauto using Promises.fulfill_minus.
+      }
+      { (* update *)
+        inv LOCAL1. inv LOCAL2. ss.
+        esplits.
+        - econs; [|econs 4]; eauto.
+          econs; s; eauto. i.
+          exploit NON_RESERVED; eauto. i. des; auto.
+          specialize (RESERVED loc). rewrite GET0 in *.
+          destruct (grsv1_src loc) eqn:GRSV_SRC; ss; try by intuition.
+          destruct (rsv1_src loc) eqn:RSV_SRC; auto.
+          eapply equal_f in RESERVES.
+          unfold BoolMap.minus in RESERVES.
+          rewrite GRSV_SRC, RSV_SRC, x0 in RESERVES. ss.
+          destruct (grsv1_tgt loc); ss.
+        - econs; ss.
+          rewrite PROMISES.
+          eauto using Promises.fulfill_minus.
+      }
+      { (* fence *)
+        inv LOCAL. ss.
+        esplits.
+        - econs; [|econs 5]; eauto. econs; ss.
+        - ss.
+      }
+      { (* failure *)
+        inv LOCAL. ss.
+        esplits.
+        - econs; [|econs 7]; eauto.
+        - ss.
+      }
+      { (* racy read *)
+        inv LOCAL. ss.
+        esplits.
+        - econs; [|econs 8]; eauto.
+          econs. eapply sim_is_racy; try eapply RACE; ss.
+        - ss.
+      }
+      { (* racy write *)
+        inv LOCAL. ss.
+        esplits.
+        - econs; [|econs 9]; eauto.
+          econs. eapply sim_is_racy; try eapply RACE; ss.
+        - ss.
+      }
+      { (* racy update *)
+        esplits.
+        - econs; [|econs 10]; eauto.
+          inv LOCAL.
+          + econs 1. ss.
+          + econs 2. ss.
+          + econs 3. eapply sim_is_racy; try eapply RACE; ss.
+        - ss.
+      }
+    Qed.
+
+    Lemma program_step_reserves
+          reserved e (th1 th2: Thread.t lang)
+          (STEP: Thread.step reserved true e th1 th2):
+      Global.reserves (Thread.global th1) = Global.reserves (Thread.global th2).
+    Proof.
+      inv STEP. inv STEP0; ss; try by (inv LOCAL; ss).
+      inv LOCAL1. inv LOCAL2. ss.
+    Qed.
+
+    Lemma certify_pf_certify_aux
+          (reserved: OptTimeMap.t)
+          th_src th_tgt loc
+          (SIM: sim_thread th_src th_tgt)
+          (RESERVED: forall loc, reserved loc <-> Global.reserves (Thread.global th_src) loc)
+          (CERTIFY: certify reserved loc th_tgt):
+      pf_certify_aux reserved loc th_src.
+    Proof.
+      inv CERTIFY.
+      { revert th_src SIM RESERVED.
+        induction STEPS; i.
+        { destruct pf; [|inv STEP_FAILURE; inv STEP; ss].
+          exploit sim_thread_program_step; try exact STEP_FAILURE; eauto.
+          { destruct e; ss. }
+          i. des.
+          econs 1; [refl|..]; eauto.
+        }
+        inv H. inv STEP. destruct pf0.
+        { exploit sim_thread_program_step; try exact STEP0; eauto; try apply EVENT. i. des.
+          exploit IHSTEPS; eauto.
+          { i. erewrite <- program_step_reserves; eauto. }
+          i. inv x1.
+          - econs 1; try exact STEP_FAILURE0; eauto.
+            econs 2; eauto. econs; eauto. apply EVENT.
+          - econs 2; try exact STEP_FULFILL; eauto.
+            econs 2; eauto. econs; eauto. apply EVENT.
+        }
+        { eauto using sim_thread_internal_step. }
+      }
+      { revert th_src SIM RESERVED.
+        induction STEPS; i.
+        { destruct pf; [|inv STEP_FULFILL; inv STEP; ss].
+          exploit sim_thread_program_step; try exact STEP_FAILURE; eauto.
+          { destruct e; ss. }
+          i. des.
+          econs 2; [refl|..]; eauto.
+          inv SIM. congr.
+        }
+        inv H. inv STEP. destruct pf0.
+        { exploit sim_thread_program_step; try exact STEP0; eauto; try apply EVENT. i. des.
+          exploit IHSTEPS; eauto.
+          { i. erewrite <- program_step_reserves; eauto. }
+          i. inv x1.
+          - econs 1; try exact STEP_FAILURE; eauto.
+            econs 2; eauto. econs; eauto. apply EVENT.
+          - econs 2; try exact STEP_FULFILL0; eauto.
+            econs 2; eauto. econs; eauto. apply EVENT.
+        }
+        { eauto using sim_thread_internal_step. }
+      }
+    Qed.
+
+    Lemma certify_pf_certify
+          th loc
+          (CERTIFY: certify (Global.max_reserved (Thread.global th)) loc th):
+      pf_certify loc th.
+    Proof.
+      exploit certify_pf_certify_aux; try exact CERTIFY; try refl.
+      { i. unfold Global.max_reserved, Memory.max_opt_timemap. condtac; ss. }
+      i. inv x0.
+      - econs 1; eauto.
+      - econs 2; eauto.
+    Qed.
+
+    Lemma consistent_pf_certify
+          th loc
+          (LC_WF: Local.wf (Thread.local th) (Thread.global th))
+          (GL_WF: Global.wf (Thread.global th))
+          (CONS: Thread.consistent th)
+          (PROMISED: th.(Thread.local).(Local.promises) loc = true):
+      pf_certify loc th.
+    Proof.
+      apply certify_pf_certify; auto.
+      apply non_sc_consistent_certify; auto.
+      apply consistent_non_sc_consistent; auto.
+    Qed.
+  End PFCertify.
 End PFCertify.
